\documentclass{report}

\input{header.tex}

\begin{document}

Given a set based S-Category $\C$ which is a model of the non-polymorphic effect calculus, we generate an indexed category capable of modelling the polymorphic effect calculus.
\section{The Non-Polymorphic Model}
Since $\C$ is a model of the non-polymorphic calculus,
\begin{itemize}
    \item $\C$ is cartesian closed.
    \item $\C$ has a strong graded monad: $\Tz{}{}: (E, \dot, \subeffect_0, \1) \rightarrow [\C, \C]$
    \item $\C$ has a co-product on the terminal object $\1$.
\end{itemize}

In addition, we require that 
\begin{itemize}
    \item $\C$ should be complete (e.g a sub-category of $\set$)
    \item $E$ should be small.
\end{itemize}


\section{Base Category}

We construct the base category, $\Eff$ as follows:

\begin{itemize}
    \item $U = E$, the set of ground effects in the non-polymorphic language.
    \item $\1$ is a singleton set.
    \item $U^n = E^n$, set of $n$-wide tuples of effects, $\vec{\e}$
\end{itemize}

Hence when we treat effects that are well formed in $\P$ as morphisms, $E^n \rightarrow E$ in $\Eff$, we should treat them as functions $f: E^n \rightarrow E$. Ground effects become point functions: $e: \1 \rightarrow E$, so the denotation of a ground effect is the constant value function: $\deno{\typerelation{\P}{e}{\effect}} = \ev \mapsto e$

We extend the multiplication of ground effects to multiplication on effect functions, giving us our $\Mul$ operation

\begin{align}
    \Mul(f, g) & = f\dot g\\
    (f\dot g)(\ev) & = (f\ev)\dot(g\ev)\\
\end{align}

This satisfies naturality of $\Mul$.

\begin{equation}
    ((f\dot g)\after \theta)\ev = (f(\theta\ev))\dot(g(\theta\ev)) = ((f\after\theta)\dot(g\after\theta))\ev
\end{equation}

\section{S-Categories}
The semantic category, $\C_0$ of the effect-environment $\nil$ is $\C$.

Since each effect-environment is alpha equivalent to a natural number, the semantic category for $\P$ shall be represented as $\C_{\P} = \C_n = [E^n, \C]$, the category of functions $E^n\rightarrow \C$.

Objects in $[E^n, \C]$ are functions and we describe them by their actions on a generic vector of ground effects, $\ev$.

Morphisms in $[E^n, \C]$ are natural transformations between the functions. So:

\begin{align}
    m:\quad&A \rightarrow B \qt{ In $[E^n, \C]$}\\
    m\ev:\quad& A\ev \rightarrow B\ev \qt{In $\C$}\\
    (f\after g)\ev =\quad& (f\ev)\after(g\ev)\\
    \1(\ev) =\quad& \1
\end{align}

So morphisms are dependently typed functions from a vector of ground effects to morphisms in $\C$.
\subsection{Each S-Category is a CCC}
Since $\C$ is complete and a CCC, and $E^n$ is small, since $E$ is small, $[E^n, \C]$ is a CCC.

\begin{align}
    (A\times B)\ev & = (A\ev)\times(B\ev)\\
    \1\ev & = \1\\
    (B^A)\ev &= (B\ev)^{(A\ev)}\\
    \p\ev & = \p\\
    \pp\ev & = \pp\\
    \app\ev & = \app\\
    \cur{f}\ev & = \cur{f\ev}\\
    \pr{f}{g}\ev & = \pr{f\ev}{g\ev}\\
\end{align}

\subsection{The Terminal Co-Product}

We can define the co-product point-wise.

\begin{align}
    (\1 + \1)\ev & = (\1\ev + \1\ev)\\
    & = (\1 + \1)\\
    \inl\ev &= \inl\\
    \inr\ev &= \inr\\
    [f, g]\ev &= [f\ev, g\ev]\\
\end{align}

This preserves the co-product diagram.

\begin{align}
    ([f, g]\after\inl)\ev & = [f\ev, g\ev]\after \inl\\
    & = f\ev\\
    & \square\\
    ([f, g]\after\inr)\ev& = [f\ev, g\ev]\after \inr\\
    & = f\ev\\
    & \square\\
\end{align}

Suppose $l \after \inl = f$ and $l\after \inr = g$ then $l\ev \after \inl = f\ev$ and $l\ev \after\inr = g\ev$ then by in co-product in $\C$, $l = [f\ev, g\ev]$ so $l = [f, g]$.


\subsection{Ground Types and Terms}
Each ground type in the non-polymorphic calculus has a fixed denotation $\deno{\g}\in\obj\C$. The ground type in the polymorphic calculus hence has a denotation represented by the constant function.

\begin{align}
    \deno{\g}:&\quad E^n\rightarrow \obj\C\\
    \ev \mapsto&\quad  \deno{\g}\\
\end{align}

Each constant term $\const{A}$ in the non-polymorphic calculus has a fixed denotation $\deno{\const{A}}\in\C(\1, A)$.

So the morphism $\deno{\const{A}}$ in $[E^n, \C]$ is the corresponding constant dependently typed morphism.

\begin{align}
    \deno{\const{A}}:&\quad[E^n, \C](\1, A)\\
    \ev\mapsto&\quad\deno{\const{A}}
\end{align}

\subsection{Graded Monad}
Given the strong graded monad $(\Tz{}{}, \pointz{}{}{}, \bindz{}{}{}, \tstrengthz{}{}{})$ on $\C$ we can construct an appropriate graded monad on $[E^n, \C]$.

\begin{align}
    \Tn{}{}:&\quad(E^n, \dot, \subeffect_n, \1_n) \rightarrow [[E^n, \C], [E^n, \C]]\\
    (\Tn{f}{A})\ev=&\quad \Tz{(f\ev)}{A\ev}\\
    (\pointn{A})\ev=&\quad\pointz{A\ev}\\
    (\bindn{f}{g}{A})\ev=&\quad\bindz{(f\ev)}{(g\ev)}{(A\ev)}\\
    (\tstrengthn{f}{A}{B})\ev=&\quad\tstrengthz{(f\ev)}{(A\ev)}{(B\ev)}
\end{align}

Through some mechanical proof and the naturality of the $\C$ strong graded monad, these morphisms are natural in their type parameters and form a strong graded monad in $[E^n, \C]$


\subsubsection{Naturality}

\begin{tikzcd}
    A\ev 
    \arrow{r}{\pointz{(A\ev)}}
    \arrow{d}{f\ev}
    &
    \Tz{\1}{(A\ev)}
    \arrow{d}{\Tz{\1}{(f\ev)}}
    \\
    B\ev
    \arrow{r}{\pointz{(B\ev)}}
    &
    \Tz{\1}{(B\ev)}
\end{tikzcd}

\begin{tikzcd}
    \Tz{(f\ev)}{\Tz{(g\ev)}{(A\ev)}}
    \arrow{r}{\bindz{f\ev}{g\ev}{(B\ev)}}
    \arrow{d}{\Tz{f\ev}{\Tz{g\ev}{m\ev}}}
    &
    \Tz{(f\ev)\dot(g\ev)}{(A\ev)}
    \arrow{d}{\Tz{(f\ev)\dot(g\ev)}{m\ev}}
    \\
    \Tz{(f\ev)}{\Tz{(g\ev)}{(B\ev)}}
    \arrow{r}{\bindz{f\ev}{g\ev}{(B\ev)}}
    &
    \Tz{(f\ev)\dot(g\ev)}{(A\ev)}
\end{tikzcd}


\begin{tikzcd}
    A\ev \times \Tz{f\ev}{(B\ev)}
    \arrow{r}{\tstrengthz{f\ev}{(A\ev)}{(B\ev)}}
    \arrow{d}{(m\ev\times\Id{\Tz{f\ev}{B}})}
    &
    \Tz{f\ev}{(A\ev\times B\ev)}
    \arrow{d}{\Tz{(f\ev)}{(m\ev\times \Id{B\ev})}}
    \\
    A'\ev \times \Tz{f\ev}{(B\ev)}
    \arrow{r}{\tstrengthz{f\ev}{(A'\ev)}{(B\ev)}}
    &
    \Tz{f\ev}{(A'\ev\times B\ev)}
\end{tikzcd}

\begin{tikzcd}
    A\ev \times \Tz{f\ev}{(B\ev)}
    \arrow{r}{\tstrengthz{f\ev}{(A\ev)}{(B\ev)}}
    \arrow{d}{(\Id{A\ev}\times \Tz{f\ev}{(m\ev)})}
    &
    \Tz{f\ev}{(A\ev\times B\ev)}
    \arrow{d}{\Tz{(f\ev)}{(\Id{A\ev} \times m\ev)}}
    \\
    A\ev \times \Tz{f\ev}{(B'\ev)}
    \arrow{r}{\tstrengthz{f\ev}{(A\ev)}{(B'\ev)}}
    &
    \Tz{f\ev}{(A\ev\times B'\ev)}
\end{tikzcd}


\subsubsection{Monad Laws}
\paragraph{Left Unit}

\begin{align}
    (\bindn{f}{\1}{A}\after\Tn{f}{\pointn{A}})\ev &= \bindz{(f\ev)}{\1}{(A\ev)} \after \Tz{f\ev}{(\pointz{A\ev})}\\
    &= \Id{\Tz{f\ev}{A\ev}}\\
    &=(\Id{\Tn{f}{A}})\ev
\end{align}

\paragraph{Right Unit}

\begin{align}
    (\bindn{\1}{g}{A}\after\pointn{\Tn{f}{A}})\ev &= \bindz{\1}{(f\ev)}{(A\ev)} \after (\pointz{\Tz{f\ev}{A\ev}})\\
    &= \Id{\Tz{f\ev}{A\ev}}\\
    &=(\Id{\Tn{f}{A}})\ev
\end{align}


\paragraph{Monad Associativity}

\begin{align}
    ((\bindn{f}{(g\dot h)}{A})\after\Tn{f}{(\bindn{g}{h}{A})})\ev &= \bindz{(f\ev)}{((g\ev)\dot(h\ev))}{(A\ev)}\after\Tz{f\ev}{\bindz{(h\ev)}{(g\ev)}{A\ev}}\\
    &= \bindz{((f\ev)\dot(g\ev))}{(h\ev)}{(A\ev)}\after\bindz{(f\ev)}{(g\ev)}{(\Tz{h\ev}{(A\ev)})}\\
    & = (\bindn{f\dot g}{h}{A}\after\bindn{f}{g}{\Tz{h}{A}})\ev
\end{align}
\subsubsection{Tensorial Strength}

\paragraph{Unitor Law}
\begin{align}
    (\Tn{f}{\pp})\ev&= \Tz{(f\ev)}{(\pp\ev)}\\
    & =  \Tz{(f\ev)}{(\pp)}\\
    & = \pp\\
    &= \pp\ev
\end{align}

\paragraph{Bind Law}

\begin{tikzcd}[ampersand replacement=\&]
    A \times \Tn{f}{\Tn{g}{B}} 
    \arrow [r, "\tstrength{f}{A}{\Tn{g}{B}}"]
    \arrow [dr, "\Id{A} \times \bindn{f}{g}{B}"]
    \& 
    \Tn{f}{(A \times \Tn{g}{B})} 
    \arrow [r, "\Tn{f}{\tstrength{g}{A}{B}}"]
    \& 
    \Tn{f}{\Tn{g}{(A \times B)}} 
    \arrow [d, "\bindn{f}{g}{A \times B}"]
    \\
    \&
    A \times \Tn{f \dot g}{B}  
    \arrow [r, "\tstrength{f \dot g}{A}{B}"] 
    \&
    \Tn{f \dot g}({A \times B)}
\end{tikzcd}

\begin{align}
    (\tstrengthn{(f\dot g)}{A}{B}\after (\Id{A}\times \bindn{f}{g}{B}))\ev & = (\tstrengthz{((f\ev)\dot (g\ev))}{(A\ev)}{(B\ev)}\after (\Id{A\ev}\times \bindn{(f\ev)}{(g\ev)}{(B\ev)}))\\
    & = \bindz{(f\ev)}{(g\ev)}{(A\times B)\ev}\after\Tz{f\ev}{(\tstrengthz{(g\ev)}{(A\ev)}{(B\ev)})}\after\tstrengthz{(f\ev)}{(A\ev)}{\Tz{g\ev}{(B\ev)}}\\
    & = (\bindn{f}{g}{(A\times B)}\after\Tn{f}{(\tstrengthn{g}{A}{B})}\after\tstrengthn{f}{A}{\Tn{g}{(B)}})\ev
\end{align}



\paragraph{Commutativity with Unit}

\begin{tikzcd}[ampersand replacement=\&]
    A \times B
    \arrow [r, "\Id{A} \times \point{B}"]
    \arrow [rd, "\point{A \times B}"]
    \&
    A \times \tob 
    \arrow [d, "\tstrength{\1}{A}{B}"]
    \\
    \&
    \Tn{\1}{(A \times B)}
\end{tikzcd}

\begin{align}
    (\tstrengthn{\1}{A}{B}\after(\Id{A}\times \pointn{A}))\ev & = \tstrengthz{\1}{(A\ev)}{(B\ev)}\after(\Id{A\ev}\times \pointz{A\ev})\\
    & = \pointz{A\ev\times B\ev}\\
    & = (\pointn{A\times B})\ev
\end{align}

\paragraph{Commutativity with $\alpha$}
Let $\alpha_{A, B, C} = \pr{\p\after\p}{\pr{\pp\after\p}{\pp}}: ((A \times B) \times C) \rightarrow (A \times (B \times C))$


\begin{tikzcd}[ampersand replacement=\&]
    (A\times B)\times \Tn{\e}{C} 
    \arrow [rr, "\tstrength{\e}{(A\times B)}{C}"]
    \arrow [d, "\alpha_{A, B, \Tn{\e}{C}}"]
    \& \& \Tn{\e}{((A \times B)\times C)}
    \arrow [d, "\Tn{\e}{\alpha_{A, B, C}}"]
    \\
    A \times (B \times \Tn{\e}{C}) 
    \arrow [r, "\Id{A}\times\tstrength{\e}{B}{C}"]
    \&
    A\times\Tn{\e}{(B \times C)} 
    \arrow [r, "\tstrength{\e}{A}{(B \times C)}"]
    \& \Tn{\e}{(A \times (B \times C))}
    \\
\end{tikzcd}

\begin{align}
    (\Tn{f}{\alpha_{A, B, C}}\after\tstrengthn{f}{A\times B}{C})\ev & = \Tz{f\ev}{\alpha_{A\ev, B\ev, C\ev}} \after\tstrengthz{(f\ev)}{(A\times B)\ev}{(C\ev)}\\
    & = \tstrengthz{(f\ev)}{(A\ev)}{(B\ev\times C\ev)}\after(\Id{A\ev}\times \tstrengthz{(f\ev)}{(B\ev)}{(C\ev)})\after\alpha_{A\ev, B\ev, C\ev}\\
    & = (\tstrengthn{f}{A}{(B\times C)}\after(\Id{A}\times \tstrengthn{f}{B}{C})\after\alpha_{A, B, C})\ev\\
\end{align}


\subsection{Sub-Effecting}
Given a collection of sub-effecting natural transformation in $\C$,

\begin{align}
    \deno{\e_1\subeffectz \e_2}:&\quad \Tz{\e_1}{} \rightarrow \Tz{\e_2}{}
\end{align}

We can form sub-effect natural transformations in $[E^n, \C]$:

\begin{align}
    \deno{f\subeffectn g}:&\quad\Tn{f}{}\rightarrow \Tn{g}{}\\
    \deno{f\subeffectn g} A \ev:&\quad\Tn{f\ev}{(A\ev)}\rightarrow \Tn{g\ev}{(B\ev)}\\
    =&\quad \deno{f\ev\subeffectz g\ev}A\ev
\end{align}

\subsubsection{Naturality}

\begin{tikzcd}
    \Tz{f\ev}{A\ev}
    \arrow{r}{\deno{f\ev\subeffectz g\ev}A\ev}
    \arrow{d}{\Tz{f\ev}{m\ev}}
    &
    \Tz{g\ev}{A\ev}
    \arrow{d}{\Tz{g\ev}{m\ev}}
    \\
    \Tz{f\ev}{B\ev}
    \arrow{r}{\deno{f\ev\subeffectz g\ev}B\ev}
    &
    \Tz{g\ev}{B\ev}
\end{tikzcd}

\subsubsection{Commutes With Tensor Strength}

\begin{tikzcd}[ampersand replacement=\&]
    A \times \Tn{f}{B} \arrow [r, "\Id{A} \times \dsen{f}{g}_B"] \arrow [d, "\tstrengthn{f}{A}{B}"] \&
    A \times \Tn{g}{B} \arrow [d, "\tstrengthn{g}{A}{B}"] \\
    \Tn{f}{(A \times B)} \arrow [r, "\dsen{f}{g}_{ A \times B}"] \&
    \Tn{g}{(A \times B)} 
\end{tikzcd}

\begin{align}
    (\tstrengthn{g}{A}{B}\after(\Id{A}\times \db{f\subeffectn g}_B))\ev & = \tstrengthz{(g\ev)}{(A\ev)}{(B\ev)}\after(\Id{A\ev}\times \db{f\ev \subeffectz g\ev}_{B\ev})\\
    & = \db{f\ev \subeffectz g\ev}_{(A\times B)\ev} \after\tstrengthz{(f\ev)}{(A\ev)}{(B\ev)}\\
    & = (\db{f \subeffectn g}_{(A\times B)} \after\tstrengthn{f}{A}{B})\ev\\
\end{align}

\subsubsection{Commutes with Join}

\begin{tikzcd}[ampersand replacement=\&]
    \Tn{f}{\Tn{g}{}} 
    \arrow [rr, "\Tn{f}{\deno{g\subeffectn g'}
    }"]
    \arrow [d, "\bindn{f}{g}{}"]
    \&  \&
    \Tn{f}{\Tn{g'}{}}
    \arrow [rr, "\db{f \subeffectn f'}_{M, \Tn{g'}{}}"]
    \& \&
     \Tn{f'}{\Tn{g'}{}} 
     \arrow [d, "\bindn{f'}{g'}{}"]
     \\
    \Tn{f\dot g}{}
    \arrow [rrrr, "\deno{f\dot g\subeffectn f'\dot g'}"]
    \& \&
     \& \&
    \Tn{f'\dot g'}{}
\end{tikzcd}

\begin{align}
    (\dsen{f\dot g}{f'\dot g'}_A\after\bindn{f}{g}{A})\ev & = \dsez{(f\ev)\dot(g\ev)}{(f'\ev)\dot (g\ev)}_{A\ev}\after\bindz{(f\ev)}{(g\ev)}{(A\ev)}\\
    & = \bindz{(f\ev)}{(g\ev)}{(A\ev)}\after\dsez{f\ev}{f'\ev}_{\Tz{g'\ev}{(A\ev)}}\after \Tz{f\ev}{\dsez{g\ev}{g'\ev}}_{(A\ev)}\\
    &= \bindn{f}{g}{A}\after\dsen{f}{f'}_{\Tn{g'}{A}}\after\Tn{f}{\dsen{g}{g'}}_A
\end{align}

\subsection{Sub-Typing}
Sub-typing in $[E^n, \C]$ holds via sub-typing in $\C$

\begin{align}
    \deno{A\subtype_n B}:&\quad A\rightarrow B\\
    \deno{A\subtype_n B}\ev=&\quad \deno{A\ev\subtype_0 B\ev}
\end{align}

So the subtyping relation $A \subtype B$ forms a morphism in $[E^n, \C]$

\section{Functors Between S-Categories}
For a function $\theta: E^m \rightarrow E^n$ , the re-indexing functor $\theta\star$ is defined as follows:

\begin{align}
    \theta\star:\quad& [E^n, \C] \rightarrow [E^m, \C]\\
    \theta\star(A)\emv=&\quad A(\theta (\emv))\\
    f:\quad& A \rightarrow B \in[E^n, \C]\\
    \theta\star(f)\emv =&\quad f(\theta(\emv)): A(\theta(\emv)\rightarrow B(\theta(\emv)))
\end{align}



\subsection{$\theta\star$ is S-closed.}

\subsubsection{CCC}

\begin{align}
    (\theta\star(A\times B))\ev & = (A\times B)(\theta\ev)\\
    & = (A(\theta \ev)\times B(\theta\ev))\\
    & = (\theta\star A\times \theta\star B)\ev\\
\end{align}

\begin{align}
    (\theta\star \p)\ev & = \p(\theta\ev)\\
    & = \p \qt{Constant function}\\
    & = \p\ev
\end{align}


\begin{align}
    (\theta\star \pp)\ev & = \pp(\theta\ev)\\
    & = \pp \qt{Constant function}\
    & = \pp\ev
\end{align}

\begin{align}
    (\theta\star\pr{f}{g})\ev & = (\pr{f}{g})(\theta\ev)\\
    & = \pr{f(\theta\ev)}{g(\theta\ev)}\\
    &= \pr{\theta\star f}{\theta\star g}\ev
\end{align}

\begin{align}
    (\theta\star(A^B))\ev & = (A^B)(\theta\ev)\\
     & = (A (\theta\ev))^{(B (\theta\ev))}\\
     & = (\theta\star A)^{(\theta\star B)}\ev\\
\end{align}

\begin{align}
    (\theta\star \app)\ev & = \app(\theta\ev)\\
    & = \app \qt{Constant fn}\\
    & = \app\ev
\end{align}

\begin{align}
    (\theta\star\cur{f})\ev & = \cur{f}(\theta\ev)\\
    & = \cur{f(\theta\ev)}\\
    & = \cur{\theta\star f}
\end{align}


\begin{align}
    (\theta\star \1)\ev & = \1(\theta\ev)\\
    & = \1 \\
    & = \1 \ev\\
\end{align}

\begin{align}
    (\theta\star\term{A})\ev & = \term{A}(\theta\ev)\\
    & = \term{A(\theta\ev)}\\
    & = \term{\theta\star A}\ev
\end{align}


\subsubsection{Co-Product}

\begin{align}
    (\theta\star(\1 + \1))\ev & = (\1 + \1)(\theta\ev)\\
    & = (\1 + \1)\qt{Constant function}\\
    & = (\1 + \1)\ev
\end{align}

\begin{align}
    (\theta\star\inl )\ev & = \inl(\theta\ev)\\
    & = \inl \qt{Constant Fn}\\
    & = \inl \ev
\end{align}

\begin{align}
    (\theta\star\inr )\ev & = \inr(\theta\ev)\\
    & = \inr \qt{Constant Fn}\\
    & = \inr \ev
\end{align}

\begin{align}
    (\theta\star [f, g])\ev & = [f, g](\theta\ev)\\
    & = [f (\theta\ev), g(\theta\ev)]\\
    & = [\theta\star f, \theta\star g]\ev\\
\end{align}




\subsubsection{Strong Graded Monad}
\begin{align}
    (\theta\star\Tn{f}{A})\ev & = \Tn{f}{A}(\theta\ev) \\
    & = \Tz{(f(\theta\ev))}{(A(\theta\ev))}\\
    & = (\Tm{(f\after\theta)}{\theta\star A})\ev\\
\end{align}

\begin{align}
    (\theta\star\pointn{A})\ev & = \pointn{A}(\theta\ev) \\
    & = \pointz{A(\theta\ev)}\\
    & = \pointm{\theta\star A}\ev\\
\end{align}

\begin{align}
    (\theta\star \tstrengthn{f}{A}{B})\ev & = \tstrengthn{f}{A}{B}(\theta \ev)\\
    & = \tstrengthz{(f(\theta\ev))}{(A(\theta\ev))}{(B(\theta\ev))}\\
    & = \tstrength{f\after\theta}{\theta\star A}{\theta\star B}\ev\\
\end{align}

\subsubsection{Sub-Effecting}
\begin{align}
    (\theta\star(\dsen{f}{g} A))\ev & = (\dsen{f}{g} A)(\theta \ev)\\
    & = (\dsen{f(\theta\ev)}{g(\theta\ev)}(A(\theta\ev)))\\
    & = (\dsem{\theta\star f}{\theta\star g} (\theta\star A)) \ev\\
\end{align}

\subsubsection{Ground Sub-Typing}
\begin{align}
    \theta\star(\deno{A\subtypeg B})\ev  & = \deno{A\subtypeg B}(\theta\ev)\\
    & = \deno{A\subtype B} \qt{Constant Function}\\
    & = \deno{A\subtype B} \ev\\
\end{align}

\subsection{Quantification}
We need to define $\allEn: [E^{n+1}, \C]\rightarrow[E^n, \C]$

So
\begin{align}
    (\allEn A)\env =&\quad \Pi_{\e\in E} A(\env, \e)\\
    m:&\quad A\rightarrow B\\
    (\allEn m):&\quad \allEn A\rightarrow \allEn B\\
    (\allEn m)\env =&\Pi_{\e\in E} m(\env, \e)\\
\end{align}

\subsection{Adjunction}
It is the case that:
$$\pstar \dashv \allEn$$

With unit:

\begin{align}
    \unit{A}:&\quad A \rightarrow \allEn\pstar A\\
    \unit{A}(\env)=&\quad\finpr{\Id{A(\env,e)}}{\e\in E}
\end{align}


And co-unit


\begin{align}
    \counit{B} : &\quad \pstar\allEn B \rightarrow B\\
    \counit{B}(\env, \e) =&\quad \pi_\e : \Pi_{e\in E}B(\env, \e)\rightarrow \Pi_{e\in E}B(\env, \e)
\end{align}


We then define the natural bi-jection as so:

\begin{equation}
    \bar{(-)}: [E^{n_1}, \C](\pstar A, B) \leftrightarrow [E^n,\C] (A, \allEn B): \widehat{(-)}
\end{equation}

\begin{align}
    m:&\quad \pstar A \rightarrow B\\
    \bar{m}:&\quad A\rightarrow \allEn B\\
    \bar{m}(\env) =&\quad \finpr{m(\env, \e)}{e\in E}
\end{align}


\begin{align}
    n:&\quad A \rightarrow \allEn B\\
    \widehat{n}:&\quad \pstar A\rightarrow B\\
    \widehat{n}(\env, \e_{n+1}) =&\quad\pi_\e\after g(\env)
\end{align}

\subsubsection{This is an Adjunction}
For any $g: \pstar A \rightarrow B$,

\begin{align}
    (\counit{B}\after\pstar(\bar{g}))(\env, \e_{n+1}) & = \pi_{\e_{n+1}}\after\finpr{g(\env, \e')}{\e'\in E}\\
    &= g(\env, \e_{n+1})
\end{align}

\subsection{Beck-Chevalley Condition}

For $\theta: E^m \rightarrow E^n$:
\begin{align}
    ((\theta\star\after\allEn)A)\env &= \theta\star(\allEn A)\env\\
    &= (\allEn A)(\theta(\env))\\
    &= \Pi_{\e\in E}(A(\theta(\env), \e))\\
    &= \Pi_{\e\in E}(((\theta\times \Id{U})\star A)(\env, \e))\\
    &= \allEm((\theta\times\Id{E})\star A)\env\\
    &= ((\allEm\after(\theta\times\Id{E})\star)A)\env
\end{align}

And $\bar{(\theta\times\Id{U})\star \counit{}} = \Id{\theta\star\after\allI}$.

\begin{align}
    \bar{(\theta\times\Id{U})\star \counit{A}} \ev  & = \finpr{(\theta\times\Id{U})\star\counit{A}(\ev, \e)}{\e\in E}\\
    & = \finpr{\counit{A}(\theta\ev, \e)}{e\in E}\\
    & = \finpr{\pi_\e}{\e\in E}: \Pi_{\e\in E}A(\theta\ev, \e) \rightarrow \Pi_{\e\in E}A(\theta\ev, \e)\\
    & = \Id{\Pi_{\e\in E}A(\theta\ev, \e)}\\
    & = \Id{\allII\after(\theta\times\Id{U})\star A}\ev\\
    & = \Id{\theta\star\after\allI}
\end{align}

\end{document}
