
\input{CroleSections.tex}

\newcommand\simplifiedBaseCategory{
    There are 2 distinct objects in the base category, $\C$:

\begin{itemize}
    \item $U$ - The kind of \effect
    \item $\1$ - A terminal object
\end{itemize}

And we have finite products on $U$.

\begin{itemize}
    \item $U^0 = \1$
    \item $U^{n+1} = U^n \times U$
\end{itemize}

We also have the following natural operations on morphisms in $\C$.

Let $I = U^n$.

\begin{itemize}
    \item $\Mul:\ciu\times\ciu\rightarrow\ciu$ - Generates multiplication of effects.
\end{itemize}

With naturality conditions which mean, for $\theta: U^m \rightarrow U^n (I' \rightarrow I)$,
\begin{itemize}
    \item $\Mul(\phi,\psi)\after\theta = \Mul(\phi\after\theta,\psi\after\theta)$
\end{itemize}
}

\newcommand\simplifiedWellFormedNess[0]{
    
Each instance of the well-formed-ness relation on effects, $\wellformed{\P}{\e}$ has a denotation in $\C$: \begin{equation}
    \deno{\typerelation{\P}{\e}{\effect}}: I \rightarrow U
\end{equation}

It should also be the case that \begin{equation}
    \Mul(\deno{\typerelation{\P}{\e_1}{\effect}}, \deno{\typerelation{\P}{\e_2}{\effect}}) = \deno{\typerelation{\P}{\e_1\dot\e_2}{\effect}} \in \ciu
\end{equation}

That is, $\Mul$ should be have identity $\deno{\typerelation{\P}{\1}{\effect}}$ and be associative.
}

\newcommand\simpleFibres[0]{
    Each set of morphisms $\C(I)$ corresponds to a semantic-closed (S-closed) category. That is, a category satisfying all the properties needed for the non-polymorphic language:

    \begin{itemize}
        \item Cartesian Closed
        \item Co-product of the terminal object with itself ($\1 + \1$)
        \item Ground morphisms for each ground constant ($\const{A}: \1\rightarrow A$)
        \item Partial order morphisms on ground types ($\deno{A\subtypeg} B$)
        \item \todo{Po-Monoid is over morphisms $\ciu$}A strong, monad, graded by the po-monoid $(\ciu, \Mul, \subeffectp, \deno{\1})$.
    \end{itemize}
}

\newcommand\simpleReindexingFunctors[0]{
    
For each morphism $f: I' \rightarrow I$ in $\C$, there should be a co-variant, re-indexing functor  $f\star: \C(I) \rightarrow \C(I')$, which is S-closed. That is, it preserves the S-closed properties of $\C(I)$. (See below).

$(-)\star$ should be a contra-variant functor in its $\C$ argument and co-variant in its right argument.

\begin{itemize}
    \item $(g\after f)\star(a) = f\star(\g\star(a))$
    \item $\Id{I}\star(a) = a$
    \item $f\star(\Id{A}) = \Id{f\star(A)}$
    \item $f\star(a\after b) = f\star(a)\after f\star(b)$
\end{itemize}
\subsection{Preserves Ground Types}
If $\deno{\g}\in\obj\C(I)$ then $f\star\deno{\g} = \deno{\g}\in\obj\C(I')$
\subsection{$f\star$ Preserves Products}
If $\pr{g}{h}:\C(I)(Z, X\times Y)$
Then 
\begin{align}
    f\star(X\times Y) & = f\star(X)\times f\star(Y)\\
    f\star(\pr{g}{h}) & = \pr{f\star(g)}{f\star{h}}&:\C(I')(f\star Z, f\star(X)\times f\star(Y))\\
    f\star(\p) & = \p&:\C(I')(f\star(X)\times f\star(Y), f\star(X)) \\
    f\star(\pp) &= \pp&:\C(I')(f\star(X)\times f\star(Y), f\star(Y))
\end{align}

\subsection{$f\star$ Preserves Terminal Object}
If $\Id{A}:\C(I)(A, \1)$
Then 
\begin{align}
    f\star(\1) & = \1 \\
    f\star(\term{A}) & = \term{f\star(A)}&:\C(I')(f\star A, \1)\\
\end{align}

\subsection{$f\star$ Preserves Exponentials}
\begin{align}
    f\star(Z^X) & = (f\star(Z))^{(f\star(X))}\\
     f\star(\app) &= \app&:\C(I')(f\star(Z^X)\times f\star(X), f\star(Z))\\
     f\star(\cur{g}) &= \cur{f\star(g)}&:\C(I')(f\star(Y)\times f\star(X), f\star(Z)^{f\star(X)})
\end{align}

\subsection{$f\star$ Preserves Co-product on Terminal}

\begin{align}
    f\star(\1+\1) &= \1+\1\\
    f\star(\inl)  &= \inl&:\C(I')(\1, \1+\1) \\
    f\star(\inr) &= \inr&:\C(I')(\1, \1+\1) \\
    f\star([g, h]) &= [f\star(g), f\star(h)]&:\C(I')(\1+\1, f\star(Z))
\end{align}

\subsection{$f\star$ Preserves Graded Monad}
\begin{align}
    f\star(\tea) &= \T{f\star(\e)}{f\star(A)}&:\C(I')\\
    f\star(\1) &= \1 \qt{The unit effect}\\
    f\star(\point{A}) &= \point{f\star(A)}&:\C(I')(f\star(A), f\star(\toa))\\
    f\star(\bind{\e_1}{\e_2}{A}) &= \bind{f\star(\e_1)}{f\star(\e_2)}{f\star(A)}&:\C(I')(f\star(\T{\e_1}{\T{\e_2}{A}}), f\star(\T{f\star(\e_1)\dot f\star(\e_2)}{f\star(A)}))\\
    f\star(\e_1\dot\e_2) &= f\star(\e_1)\dot f\star(\e_2)\\
\end{align}

\subsection{$f\star$ Preserves Tensor Strength}
\begin{align}
    f\star(\tstrength{\e}{A}{B}) &= \tstrength{f\star(\e)}{f\star(A)}{f\star(B)} &: \C(I')(f\star(A\times\teb), f\star(\T{\e}{(A\times B)}))
\end{align}
\subsection{$f\star$ Preserves Ground Constants}
For each ground constant $\deno{\const{A}}$ in $\C(I)$,

\begin{align}
    f\star(\deno{\const{A}}) = \const{f\star(A)} : \C(I')(\1, f\star(A))
\end{align}
\subsection{$f\star$ Preserves Ground Sub-effecting}
For ground effects $e_1, e_2$ such that $e_1\subeffect e_2$



\begin{align}
    f\star(e) & = e: \C(I')\\
    f\star\db{\e_1\subeffect e_2}_A = \db{e_1 \subeffect e_2}_{f\star(A)} &:\C(I'){f\star(\T{e_1}{A}), f\star(\T{e_2}{A})} \\
\end{align}
\subsection{$f\star$ Preserves Ground Sub-typing}
For ground types $\g_1, \g_2$ such that $\g_1\subtypeg\g_2$

\begin{align}
    f\star{\g} = \g: \C(I')(\1, \g)\\
    f\star(\deno{\g_1 \subtypeg \g_2}) & = \deno{\g_1 \subtypeg \g_2} &: \C(I')(\g_1, \g_2)\\
\end{align}

\subsection{Action on Objects}

It follows that the action of $f\star$ on an object $A$ in $\C(I)$ (i.e. a morphism $I \rightarrow U$ in $\C$) is:

\begin{equation}
    f\star(A) = A\after f: I'\rightarrow I\rightarrow W
\end{equation}
}



\newcommand\allISimple[0]{
    
We expand $\allI: \C(I\times U) \rightarrow \C(I)$ to be a functor which is right adjoint to the re-indexing functor $\pstar$.

\begin{equation}
    \bar{(\_)}: \C(I\times U)(\pstar A, B) \leftrightarrow \C(I)(A, \allI B) : \widehat{(\_)}
\end{equation}

For $A: \C(I)$, $B: \C(I\times U)$.

Hence the action of $\allI$ on a morphism $l : A\rightarrow A'$ is as follows:
\begin{eqnarray}
    \allI(l) = \bar{l\after\e_A}
\end{eqnarray}
Where $\e_A: \C(I\times U)(\pstar\allI A \rightarrow A)$ is the co-unit of the adjunction.

\subsection{Beck Chevalley Condition}
We need to be able to commute the $\allI$ functor with reindexing functors. A natural way to do this is:

\begin{align}
    \theta\star\after\allI & = \allII\after(\theta\times\Id{U})\star
\end{align}

We shall also require that the canonical natural-transformation between these functors is the identity.

That is, 

\begin{align}
    \bar{(\theta\times\Id{U})\star(\counit{})} = \Id{}: \theta\star\after\allI \rightarrow \allII\after(\theta\times\Id{U})\star\in \C(I')
\end{align}

This shall be called the Beck-Chevalley condition.

}


\newcommand\effectSubstitutionTypesSimple[0]{
        If $\si = \deno{\typerelation{\P'}{\si}{\P}}$ then $\deno{\typerelation{\P'}{A\ssi}{\type}} = \si\star\deno{\typerelation{\P}{A}{\type}}$.

\proof
By induction on the derivation on $\deno{\typerelation{\P}{A}{\type}}$. Making use of the S-Closure of the reindexing functor.

\case{Ground}
\begin{align}
    \si\star\deno{\typerelation{\P}{\g}{\type}} &= \si\star\deno{\g}\\
    & =  \deno{\g}\qt{By S-Closure}\\
    & = \deno{\typerelation{\P'}{\g\ssi}{\type}}
\end{align}

\case{Monad}
\begin{align}
    \si\star\deno{\typerelation{\P}{\mea}{\type}}\after\si & =  \si\star(\T{\deno{\typerelation{\P}{\e}{\effect}}}{\deno{\typerelation{\P}{A}{\type}}})\\
    &= \T{\si\star(\deno{\typerelation{\P}{\e}{\effect}})}{\si\star(\deno{\typerelation{\P}{A}{\type}})}\\
    & = \deno{\typerelation{\P'}{(\mea)\ssi}{\type}}
\end{align}
\case{Quantification}
    \begin{align}
        \si\star\deno{\typerelation{\P}{\all{\a}A}{\type}} & = \si\star(\allI(\deno{\typerelation{\P,\a}{A}{\type}}))\\
        & = \allI((\si\times\Id{U})\star\deno{\typerelation{\P,\a}{A}{\type}})\qt{By Beck-Chevalley}\\
        & = \allI(\deno{\typerelation{\P',\a}{A\sub{\si, \a\setto\e}}{\type}})\\
        & = \allI(\deno{\typerelation{\P',\a}{A\ssi}{\type}})\\
        & = \deno{\typerelation{\P'}{\all{\a}{A\ssi}}{\type}}\\
        & = \deno{\typerelation{\P'}{(\all{\a}{A})\ssi}{\type}}\\
    \end{align}

\case{Function}
\begin{align}
    \si\star\deno{\typerelation{\P}{\ab}{\type}} &= \si\star(\deno{\typerelation{\P}{B}{\type}}^{\deno{\typerelation{\P}{A}{\type}}})\\
    &=\si\star(\deno{\typerelation{\P}{B}{\type}})^{\si\star(\deno{\typerelation{\P}{A}{\type}})}\\
    & = \deno{\typerelation{\P'}{B\ssi}{\type}}^{\deno{\typerelation{\P'}{A\ssi}{\type}}}\\
    & = \deno{\typerelation{\P'}{\fntype{(A\ssi)}{(B\ssi)}}{\type}}\\
    & = \deno{\typerelation{\P'}{(\ab)\ssi}{\type}}\\
\end{align}
}


\newcommand\effectSubstitutionSubtypingSimple[0]{
    If $\si = \deno{\typerelation{\P'}{\si}{\P}}$ then $\deno{A\ssi\subtypepp B\ssi} = \si\star\deno{A\subtypep B}: \C(I')(A, B)$.

\proof
By induction on the derivation on $\deno{A\subtypep B}$. Using S-closure of $\si\star$ 

\case{Ground}
\begin{align}
    \si\star(\g_1\subtypeg\g_2) &= (\g_1\subtypeg\g_2)
\end{align}

Since $\si\star$ is s-closed.

\case{Monad}
\begin{align}
    \si\star\deno{\M{\e_1}{A} \subtypep \M{\e_2}{B}} & = \si\star(\deno{\e_1\subeffectp\e_2})\after\si\star(\T{\e_1}(\deno{A\subtypep B})) \\ 
     &= \deno{\si(\e_1)\subeffectpp\si(\e_2)} \after \T{\si(\e_1)}{\deno{A\ssi\subtypepp B\ssi}}\qt{By S-Closure}\\
     &= \deno{\M{\si(\e_1)}{A\ssi}\subtypepp\M{\si(\e_2)}{B\ssi}}\\
     &= \deno{(\M{\e_1}{A})\ssi\subtypepp\M{\e_2}{B}\ssi}\\
\end{align}

\case{For All}
    \begin{align}
        \si\star\deno{\all{\a}{A}\subtypep\all{\a}{B}} &= \si\star(\allI(\deno{A\subtypepa B})) \\
        &=\allII((\si\times\Id{U})\star(\deno{A\subtypepa B}))\\
        &=\allII(\deno{A\sub{\si,\a\setto\a}\subtypeppa B\sub{\si,\a\setto\a}})\\
        &= \deno{(\all{\a}{A})\ssi \subtypepp(\all{\a}{B})\ssi}\\
    \end{align}

\case{Fn}
\begin{align}
    \si\star\deno{(\ab)\subtypep\fntype{A'}{B'}} &= \si\star(\deno{B\subtypep B'}^{A'}\after B^{\deno{A'\subtypep A}})\\
    &= \si\star(\cur{\deno{B\subtypep B'}\after\app})\after\si\star(\cur{\app\after(\Id{B}\times\deno{A'\subtypep A})})\\
    & = \cur{\si\star(\deno{B\subtypep B'})\after\app}\after\cur{\app\after(\Id{B}\times\si\star(\deno{A'\subtypep A}))}\\
    & = \cur{\deno{B\ssi\subtypepp B'\ssi}\after\app}\after\cur{\app\after(\Id{B\ssi}\times\deno{A'\ssi\subtypepp A\ssi})}\\
    &= \deno{\fntype{(A\ssi)}{(B\ssi)}\subtypepp\fntype{(A'\ssi)}{(B'\ssi)}}\\
    &= \deno{(\ab)\ssi\subtypepp(\fntype{A'}{B'})\ssi}
\end{align}

}


\newcommand\typeDenotationsSimple[0]{
    
For each instance of the well-formed-ness relation on types, we derive an object $\deno{\typerelation{\P}{A}{\type}}\in\obj\C(I)$.

Since the fibre category $\C(I)$ is S-Closed, it has objects for all ground types, a terminal object, graded monad $\T{}{}$, exponentials, products, and co-product over $\1+\1$.

\begin{itemize}
    \item $\deno{\typerelation{\P}{\U}{\type}} = \1$
    
    \item $\deno{\typerelation{\P}{\B}{\type}} = \1+\1$
    
    \item $\deno{\typerelation{\P}{\g}{\type}} = \deno{\g} $
    
    \item $\deno{\typerelation{\P}{\ab}{\type}} = (\deno{\typerelation{\P}{B}{\type}})^{(\deno{\typerelation{\P}{A}{\type}})}$
    
    \item $\deno{\typerelation{\P}{\mea}{\type}} =\T{\deno{\typerelation{\P}{\e}{\effect}}}{\deno{\typerelation{\P}{A}{\type}}}$
    \item $\deno{\typerelation{\P}{\all{\a}{A}}{\type}} =\allI(\deno{\typerelation{\P,\a}{A}{\type}})$
\end{itemize}
}


\newcommand\subtypingDenotationsSimple[0]{
    
For each instance of the sub-typing relation with respect  to an effect environment, there exists a denotation, $\deno{A\subtypep B}: \C(I)(A, B)$.

\begin{itemize}
    \item $\deno{\g_1\subtypep \g_2} = \deno{\g_1\subtypeg \g_2} : \C(I)(\g_1, \g_2)$
    \item $\deno{\ab \subtypep \fntype{A'}{B'}} = \deno{B\subtypep B'}^{A'}\after B^{\deno{A'\subtypep A}}$
    \item $\deno{\M{\e_1}{A}\subtypep\M{\e_2}{B}} = \deno{\e_1\subeffectp\e_2}\after\T{\e_1}{\deno{A\subtypep B}}$
    \item $\deno{\all{\a}{A}\subtypep\all{\a}{B}} = \allI{\deno{A\subtypepa B}}$
\end{itemize}
}


\newcommand{\typeEnvDenotationsSimple}[0]{
    

For each instance of the well-formed relation on type environments, define an object $\deno{\wellformedok{\P}{\G}}\in\obj\C(I)$.

\begin{itemize}
    \item $\deno{\wellformedok{\P}{\nil}} = \1: \C(I)$
    \item $\deno{\wellformedok{\P}{\gax}} = (\deno{\wellformedok{\P}{\G}} \times \deno{\typerelation{\P}{A}{\type}})$
\end{itemize}

}


\newcommand\effectSubstitutionTypeEnvsSimple[0]{
    
If $\si = \deno{\typerelation{\P'}{\si}{\P}}$ then $\deno{\wellformedok{\P'}{\G\ssi}} = \si\star\deno{\wellformedok{\P}{\G}}\in\obj\C(I')$.

\proof
By induction on the derivation on $\deno{\wellformedok{\P}{\G}}$. Using the S-Closure of the re-indexing functor.

\case{Nil}
\begin{align}
    \si\star\deno{\wellformedok{\P}{\nil}} &=\si\star\1\\
    & = \1\qt{By S-closure}\\
    &= \deno{\wellformedok{\P'}{\nil}}\\
    &= \deno{\wellformedok{\P'}{\nil\ssi}}\\
\end{align}

\case{Var}
\begin{align}
   \si\star\deno{\wellformedok{\P}{\gax}} &= \si\star(\deno{\wellformedok{\P}{\G}} \times \deno{\typerelation{\P}{A}{\type}}) \\
   & = (\si\star\deno{\wellformedok{\P}{\G}} \times \si\star\deno{\typerelation{\P}{A}{\type}})\\
    & = (\deno{\wellformedok{\P'}{\G\ssi}} \times \deno{\typerelation{\P'}{A\ssi}{\type}})\\
    & = \deno{\wellformedok{\P'}{\G\ssi, x: A\ssi}}\\
    & = \deno{\wellformedok{\P'}{(\gax)\ssi}}\\
\end{align}
}


\newcommand\effectWeakeningTypesSimple[0]{
    If $\w = \deno{\typerelation{\P'}{\w}{\P}}$ then $\deno{\typerelation{\P'}{A}{\type}} = \w\star\deno{\typerelation{\P}{A}{\type}}$.
    
    \proof
    By induction on the derivation on $\deno{\typerelation{\P}{A}{\type}}$. Making use of the S-Closure of the reindexing functor.
    
    \case{Ground}
    \begin{align}
        \w\star\deno{\typerelation{\P}{\g}{\type}} &= \w\star\deno{\g}\\
        & =  \deno{\g}\qt{By S-Closure}\\
        & = \deno{\typerelation{\P'}{\g}{\type}}
    \end{align}
    
    \case{Monad}
    \begin{align}
        \w\star\deno{\typerelation{\P}{\mea}{\type}}\after\w & =  \w\star(\T{\deno{\typerelation{\P}{\e}{\effect}}}{\deno{\typerelation{\P}{A}{\type}}})\\
        &= \T{\w\star(\deno{\typerelation{\P}{\e}{\effect}})}{\w\star(\deno{\typerelation{\P}{A}{\type}})}\\
        & = \deno{\typerelation{\P'}{\mea}{\type}}
    \end{align}
    \case{Quantification}
        \begin{align}
            \w\star\deno{\typerelation{\P}{\all{\a}A}{\type}} & = \w\star(\allI(\deno{\typerelation{\P,\a}{A}{\type}}))\\
            & = \allI((\w\times\Id{U})\star\deno{\typerelation{\P,\a}{A}{\type}})\qt{By Beck-Chevalley}\\
            & = \allI(\deno{\typerelation{\P',\a}{A}{\type}})\\
            & = \allI(\deno{\typerelation{\P',\a}{A}{\type}})\\
            & = \deno{\typerelation{\P'}{\all{\a}{A}}{\type}}\\
        \end{align}
    
    \case{Function}
    \begin{align}
        \w\star\deno{\typerelation{\P}{\ab}{\type}} &= \w\star(\deno{\typerelation{\P}{B}{\type}}^{\deno{\typerelation{\P}{A}{\type}}})\\
        &=\w\star(\deno{\typerelation{\P}{B}{\type}})^{\w\star(\deno{\typerelation{\P}{A}{\type}})}\\
        & = \deno{\typerelation{\P'}{B}{\type}}^{\deno{\typerelation{\P'}{A}{\type}}}\\
        & = \deno{\typerelation{\P'}{\ab}{\type}}\\
    \end{align}
}

\newcommand\effectWeakeningTypeEnvSimple[0]{
    
If $\w = \deno{\typerelation{\P'}{\w}{\P}}$ then $\deno{\wellformedok{\P'}{\G}} = \w\star\deno{\wellformedok{\P}{\G}}\in\obj\C(I')$.

\proof
By induction on the derivation on $\deno{\wellformedok{\P}{\G}}$. Using the S-Closure of the re-indexing functor.

\case{Nil}
\begin{align}
    \w\star\deno{\wellformedok{\P}{\nil}} &=\w\star\1\\
    & = \1\qt{By S-closure}\\
    &= \deno{\wellformedok{\P'}{\nil}}\\
\end{align}

\case{Var}
\begin{align}
   \w\star\deno{\wellformedok{\P}{\gax}} &= \w\star(\deno{\wellformedok{\P}{\G}} \times \deno{\typerelation{\P}{A}{\type}}) \\
   & = (\w\star\deno{\wellformedok{\P}{\G}} \times \w\star\deno{\typerelation{\P}{A}{\type}})\\
    & = (\deno{\wellformedok{\P'}{\G}} \times \deno{\typerelation{\P'}{A}{\type}})\\
    & = \deno{\wellformedok{\P'}{\G, x: A}}\\
\end{align}
}
